revisiting total correctness
git-svn-id: orca@275

WP1-Programming-Languages-Semantics/WP11-C-semantics/src/IMP-Lenses/theories/utp_fault_designs.thy
@@ -15,7 +15,9 @@ text {*In order to record the interaction of a sequential C program with its exe
 
 alphabet 'f cp_vars = des_vars +
   abrupt:: bool
-  fault :: "'f option"
+  fault :: bool
+  fault_tr :: "'f option"
+  stuck :: bool
   (*wait :: bool*)
 
 declare cp_vars.splits [alpha_splits]
@@ -32,14 +34,15 @@ text {*
 *}
 
 interpretation cp_vars:
-  lens_interp "\<lambda> (ok, r) . (ok, fault\<^sub>v r, abrupt\<^sub>v r, (*wait\<^sub>v r,*)more r)"
+  lens_interp "\<lambda> (ok, r) . (ok, abrupt\<^sub>v r, fault\<^sub>v r, fault_tr\<^sub>v r, stuck\<^sub>v r, more r)"
 apply (unfold_locales)
 apply (rule injI)
 apply (clarsimp)
 done
 
 interpretation cp_vars_rel: lens_interp "\<lambda>(ok, ok', r, r').
-  (ok, ok', fault\<^sub>v r, fault\<^sub>v r', abrupt\<^sub>v r, abrupt\<^sub>v r', (*wait\<^sub>v r, wait\<^sub>v r',*) more r, more r')"
+  (ok, ok', abrupt\<^sub>v r, abrupt\<^sub>v r', fault\<^sub>v r, fault\<^sub>v r', fault_tr\<^sub>v r, fault_tr\<^sub>v r', stuck\<^sub>v r, 
+   stuck\<^sub>v r',more r, more r')"
 apply (unfold_locales)
 apply (rule injI)
 apply (clarsimp)
@@ -70,13 +73,16 @@ translations
    "_svid_st_a" => "CONST cp_vars_child_lens\<^sub>a"
 
 lemma cvars_ord [usubst]:
-  "$fault \<prec>\<^sub>v $fault\<acute>" "$abrupt \<prec>\<^sub>v $abrupt\<acute>"  "$ok \<prec>\<^sub>v $ok\<acute>"
-  (*"$ok \<prec>\<^sub>v $wait\<acute>" "$ok \<prec>\<^sub>v $wait" "$ok\<acute> \<prec>\<^sub>v $wait\<acute>"  "$ok\<acute> \<prec>\<^sub>v $wait"*)
-  "$ok \<prec>\<^sub>v $fault\<acute>" "$ok \<prec>\<^sub>v $fault" "$ok\<acute> \<prec>\<^sub>v $fault\<acute>"  "$ok\<acute> \<prec>\<^sub>v $fault"
-  "$ok \<prec>\<^sub>v $abrupt\<acute>" "$ok \<prec>\<^sub>v $abrupt" "$ok\<acute> \<prec>\<^sub>v $abrupt\<acute>"  "$ok\<acute> \<prec>\<^sub>v $abrupt" 
-  "$fault \<prec>\<^sub>v $abrupt\<acute>" "$fault \<prec>\<^sub>v $abrupt" "$fault\<acute> \<prec>\<^sub>v $abrupt\<acute>"  "$fault\<acute> \<prec>\<^sub>v $abrupt"
-  (*"$fault \<prec>\<^sub>v $wait\<acute>" "$fault \<prec>\<^sub>v $wait" "$fault\<acute> \<prec>\<^sub>v $wait\<acute>"  "$fault\<acute> \<prec>\<^sub>v $wait"
-  "$abrupt \<prec>\<^sub>v $wait\<acute>" "$abrupt \<prec>\<^sub>v $wait" "$abrupt\<acute> \<prec>\<^sub>v $wait\<acute>"  "$abrupt\<acute> \<prec>\<^sub>v $wait" *)
+  "$ok \<prec>\<^sub>v $ok\<acute>" "$abrupt \<prec>\<^sub>v $abrupt\<acute>" "$fault \<prec>\<^sub>v $fault\<acute>" "$fault_tr \<prec>\<^sub>v $fault_tr\<acute>" "$stuck \<prec>\<^sub>v $stuck\<acute>" 
+  "$ok \<prec>\<^sub>v $abrupt\<acute>" "$ok \<prec>\<^sub>v $abrupt" "$ok\<acute> \<prec>\<^sub>v $abrupt\<acute>" "$ok\<acute> \<prec>\<^sub>v $abrupt" 
+  "$ok \<prec>\<^sub>v $fault\<acute>" "$ok \<prec>\<^sub>v $fault" "$ok\<acute> \<prec>\<^sub>v $fault\<acute>" "$ok\<acute> \<prec>\<^sub>v $fault"
+  "$ok \<prec>\<^sub>v $fault_tr\<acute>" "$ok \<prec>\<^sub>v $fault_tr" "$ok\<acute> \<prec>\<^sub>v $fault_tr\<acute>" "$ok\<acute> \<prec>\<^sub>v $fault_tr"
+  "$ok \<prec>\<^sub>v $stuck\<acute>" "$ok \<prec>\<^sub>v $stuck" "$ok\<acute> \<prec>\<^sub>v $stuck\<acute>" "$ok\<acute> \<prec>\<^sub>v $stuck"
+  "$abrupt \<prec>\<^sub>v $fault" "$abrupt \<prec>\<^sub>v $fault\<acute>" "$abrupt\<acute> \<prec>\<^sub>v $fault" "$abrupt\<acute> \<prec>\<^sub>v $fault\<acute>"
+  "$abrupt \<prec>\<^sub>v $fault_tr" "$abrupt \<prec>\<^sub>v $fault_tr\<acute>" "$abrupt\<acute> \<prec>\<^sub>v $fault_tr" "$abrupt\<acute> \<prec>\<^sub>v $fault_tr\<acute>"
+  "$abrupt \<prec>\<^sub>v $stuck\<acute>" "$abrupt \<prec>\<^sub>v $stuck" "$abrupt\<acute> \<prec>\<^sub>v $stuck\<acute>" "$abrupt\<acute> \<prec>\<^sub>v $stuck"  
+  "$fault \<prec>\<^sub>v $stuck\<acute>" "$fault \<prec>\<^sub>v $stuck" "$fault\<acute> \<prec>\<^sub>v $stuck\<acute>" "$fault\<acute> \<prec>\<^sub>v $stuck"
+  "$fault_tr \<prec>\<^sub>v $stuck\<acute>" "$fault_tr \<prec>\<^sub>v $stuck" "$fault_tr\<acute> \<prec>\<^sub>v $stuck\<acute>" "$fault_tr\<acute> \<prec>\<^sub>v $stuck"
   by (simp_all add: var_name_ord_def)
 
 abbreviation abrupt_f::"('f, '\<alpha>, '\<beta>) rel_cp \<Rightarrow> ('f, '\<alpha>, '\<beta>) rel_cp"
@@ -85,13 +91,33 @@ where "abrupt_f R \<equiv> R\<lbrakk>false/$abrupt\<rbrakk>"
 abbreviation abrupt_t::"('f, '\<alpha>, '\<beta>) rel_cp \<Rightarrow> ('f, '\<alpha>, '\<beta>) rel_cp"
 where "abrupt_t R \<equiv> R\<lbrakk>true/$abrupt\<rbrakk>"
 
+abbreviation fault_f::"('f, '\<alpha>, '\<beta>) rel_cp \<Rightarrow> ('f, '\<alpha>, '\<beta>) rel_cp"
+where "fault_f R \<equiv> R\<lbrakk>false/$fault\<rbrakk>"
+
+abbreviation fault_t::"('f, '\<alpha>, '\<beta>) rel_cp \<Rightarrow> ('f, '\<alpha>, '\<beta>) rel_cp"
+where "fault_t R \<equiv> R\<lbrakk>true/$fault\<rbrakk>"
+
+abbreviation stuck_f::"('f, '\<alpha>, '\<beta>) rel_cp \<Rightarrow> ('f, '\<alpha>, '\<beta>) rel_cp"
+where "stuck_f R \<equiv> R\<lbrakk>false/$stuck\<rbrakk>"
+
+abbreviation stuck_t::"('f, '\<alpha>, '\<beta>) rel_cp \<Rightarrow> ('f, '\<alpha>, '\<beta>) rel_cp"
+where "stuck_t R \<equiv> R\<lbrakk>true/$stuck\<rbrakk>"
+
 syntax
   "_abrupt_f"  :: "logic \<Rightarrow> logic" ("_\<^sub>a\<^sub>f" [1000] 1000)
   "_abrupt_t"  :: "logic \<Rightarrow> logic" ("_\<^sub>a\<^sub>t" [1000] 1000)
+  "_fault_f"  :: "logic \<Rightarrow> logic" ("_\<^sub>f\<^sub>f" [1000] 1000)
+  "_fault_t"  :: "logic \<Rightarrow> logic" ("_\<^sub>f\<^sub>t" [1000] 1000)
+  "_stuck_f"  :: "logic \<Rightarrow> logic" ("_\<^sub>s\<^sub>f" [1000] 1000)
+  "_stuck_t"  :: "logic \<Rightarrow> logic" ("_\<^sub>s\<^sub>t" [1000] 1000)
 
 translations
   "P \<^sub>a\<^sub>f" \<rightleftharpoons> "CONST usubst (CONST subst_upd CONST id (CONST ivar CONST abrupt) false) P"
   "P \<^sub>a\<^sub>t" \<rightleftharpoons> "CONST usubst (CONST subst_upd CONST id (CONST ivar CONST abrupt) true) P"
+  "P \<^sub>f\<^sub>f" \<rightleftharpoons> "CONST usubst (CONST subst_upd CONST id (CONST ivar CONST fault) false) P"
+  "P \<^sub>f\<^sub>t" \<rightleftharpoons> "CONST usubst (CONST subst_upd CONST id (CONST ivar CONST fault) true) P"
+  "P \<^sub>s\<^sub>f" \<rightleftharpoons> "CONST usubst (CONST subst_upd CONST id (CONST ivar CONST stuck) false) P"
+  "P \<^sub>s\<^sub>t" \<rightleftharpoons> "CONST usubst (CONST subst_upd CONST id (CONST ivar CONST stuck) true) P"
 
 subsection {*UTP-Relations lift and drop*}
 
@@ -114,70 +140,74 @@ lemma unrest_ok_lift_rea [unrest]:
   "$ok \<sharp> \<lceil>P\<rceil>\<^sub>C" "$ok\<acute> \<sharp> \<lceil>P\<rceil>\<^sub>C"
   by (pred_auto)+
 
-lemma unrest_wait_lift_rea [unrest]:
+lemma unrest_abrupt_lift_rea [unrest]:
   "$abrupt \<sharp> \<lceil>P\<rceil>\<^sub>C" "$abrupt\<acute> \<sharp> \<lceil>P\<rceil>\<^sub>C"
   by (pred_auto)+
 
-lemma unrest_tr_lift_rea [unrest]:
+lemma unrest_fault_lift_rea [unrest]:
   "$fault \<sharp> \<lceil>P\<rceil>\<^sub>C" "$fault\<acute> \<sharp> \<lceil>P\<rceil>\<^sub>C"
   by (pred_auto)+
 
-lemma seqr_wait_true [usubst]: "(P ;; Q) \<^sub>a\<^sub>t = (P \<^sub>a\<^sub>t ;; Q)"
+lemma unrest_stuck_lift_rea [unrest]:
+  "$stuck \<sharp> \<lceil>P\<rceil>\<^sub>C" "$stuck\<acute> \<sharp> \<lceil>P\<rceil>\<^sub>C"
+  by (pred_auto)+
+
+lemma seqr_abrupt_true [usubst]: "(P ;; Q) \<^sub>a\<^sub>t = (P \<^sub>a\<^sub>t ;; Q)"
   by (rel_auto)
 
-lemma seqr_wait_false [usubst]: "(P ;; Q) \<^sub>a\<^sub>f = (P \<^sub>a\<^sub>f ;; Q)"
+lemma seqr_abrupt_false [usubst]: "(P ;; Q) \<^sub>a\<^sub>f = (P \<^sub>a\<^sub>f ;; Q)"
   by (rel_auto)
 
-subsection {*exec semantics*}
-text {*We introduce an execution semantics for the designs containing a specific values for 
-       the auxiliary variables composing C-program alphabet. Under this execution function
-       we consider only \emph{stable} input state ie., normal input state. 
-       Since Simpl semantics is defined only for input normal state, we will have an 
-       equivalent semantics as the one of Simpl language.*}
+lemma seqr_fault_true [usubst]: "(P ;; Q) \<^sub>f\<^sub>t = (P \<^sub>f\<^sub>t ;; Q)"
+  by (rel_auto)
 
-definition exec:: "('f,'\<alpha>,'\<beta>) rel_cp \<Rightarrow> ('f,'\<alpha>,'\<beta>) rel_cp" 
-where [urel_defs]:"exec prog = (prog =\<^sub>u $ok) "
+lemma seqr_fault_false [usubst]: "(P ;; Q) \<^sub>f\<^sub>f = (P \<^sub>f\<^sub>f ;; Q)"
+  by (rel_auto)
+
+lemma seqr_stuck_true [usubst]: "(P ;; Q) \<^sub>s\<^sub>t = (P \<^sub>s\<^sub>t ;; Q)"
+  by (rel_auto)
+
+lemma seqr_stuck_false [usubst]: "(P ;; Q) \<^sub>s\<^sub>f = (P \<^sub>s\<^sub>f ;; Q)"
+  by (rel_auto)
+
 subsection{*Healthiness conditions*}
 
-text {*Programs in abrupt state do not progress*}
-definition C3a_def [upred_defs]: "C3a(P) = (P \<triangleleft> \<not>$abrupt \<triangleright> II)"
-
-text {*Programs in fault state do not progress*}
-definition C3b_def [upred_defs]: "C3b(P) = (P \<triangleleft> $fault =\<^sub>u \<guillemotleft>None\<guillemotright> \<triangleright> II)"
-
-text {*Programs in fault or abrupt state do not progress*}
-definition C3_def [upred_defs]: "C3(P) = (P \<triangleleft> \<not>$abrupt \<and> $fault =\<^sub>u \<guillemotleft>None\<guillemotright> \<triangleright> II)"
+text {*Programs in fault or abrupt or stuck state do not progress*}
+definition C3_def [upred_defs]: 
+  "C3(P) = (P \<triangleleft> \<not>$abrupt \<and> \<not>$fault \<and> \<not>$stuck \<and> $fault_tr =\<^sub>u \<guillemotleft>None\<guillemotright> \<triangleright> II)"
 
 subsection{*Control flow statements*}
 
 text{*We introduce the known control-flow statements for C. Our semantics is restricted
-      to @{const exec}. In other words It assumes:
+      to @{const C3}. In other words It assumes:
      \begin{itemize}   
        \<^item>  an execution starting from initial stable state ie,@{term "$ok"},   
        \<^item>  terminates a final state ie,@{term "$ok\<acute>"},
        \<^item>  the final state is a normal state ie,
-          @{term "\<not>$abrupt"} and @{term "$fault =\<^sub>u \<guillemotleft>None\<guillemotright>"},
+          @{term "\<not>$abrupt"} and @{term "$fault_tr =\<^sub>u \<guillemotleft>None\<guillemotright>"},
      \end{itemize}
     Thus it capture Simpl semantics.
     *}
 
 abbreviation
- "Simpl P \<equiv> C3(true \<turnstile> (P))"
+ "Simpl P \<equiv> C3(\<lceil>true\<rceil>\<^sub>C \<turnstile> (P))"
 
 definition skip_c :: "('f,'\<alpha>) hrel_cp" ("SKIP")
-where [urel_defs]:"SKIP = Simpl (\<not>$abrupt\<acute> \<and> $fault\<acute> =\<^sub>u \<guillemotleft>None\<guillemotright> \<and> \<lceil>II\<rceil>\<^sub>C)"
+where [urel_defs]:
+  "SKIP = Simpl (\<not>$abrupt\<acute> \<and> \<not>$stuck\<acute> \<and> \<not>$fault\<acute> \<and> $fault_tr\<acute> =\<^sub>u \<guillemotleft>None\<guillemotright> \<and> \<lceil>II\<rceil>\<^sub>C)"
 
 definition stuck_c :: "('f,'\<alpha>) hrel_cp" ("STUCK")
-where [urel_defs]: "STUCK = (\<not>$ok\<acute> \<or>  $fault\<acute> \<noteq>\<^sub>u \<guillemotleft>None\<guillemotright>)"
+where [urel_defs]: "STUCK = C3($stuck\<acute>)"
 
 definition assigns_c :: "'\<alpha> usubst \<Rightarrow> ('f,'\<alpha>) hrel_cp" ("\<langle>_\<rangle>\<^sub>C")
-where [urel_defs]: "assigns_c \<sigma> = 
-                    C3(\<lceil>true\<rceil>\<^sub>D \<turnstile> (\<not>$abrupt\<acute> \<and> $fault\<acute> =\<^sub>u \<guillemotleft>None\<guillemotright> \<and> \<lceil>\<langle>\<sigma>\<rangle>\<^sub>a\<rceil>\<^sub>C))"
+where [urel_defs]: 
+  "assigns_c \<sigma> =  C3(\<lceil>true\<rceil>\<^sub>C \<turnstile> (\<not>$abrupt\<acute> \<and> \<not>$stuck\<acute> \<and> \<not>$fault\<acute> \<and> $fault_tr\<acute> =\<^sub>u \<guillemotleft>None\<guillemotright> \<and> \<lceil>\<langle>\<sigma>\<rangle>\<^sub>a\<rceil>\<^sub>C))"
 
 subsection{*THROW*}
 
 definition throw_c :: "('f,'\<alpha>) hrel_cp" ("THROW")
-where [urel_defs]: "THROW = Simpl ($abrupt\<acute> \<and> $fault\<acute> =\<^sub>u \<guillemotleft>None\<guillemotright> \<and> \<lceil>II\<rceil>\<^sub>C)"
+where [urel_defs]: 
+  "THROW = Simpl ($abrupt\<acute> \<and> \<not>$stuck\<acute> \<and> \<not>$fault\<acute> \<and> $fault_tr\<acute> =\<^sub>u \<guillemotleft>None\<guillemotright> \<and> \<lceil>II\<rceil>\<^sub>C)"
 
 subsection{*Conditional*}
 
@@ -186,8 +216,9 @@ abbreviation If_c :: "'\<alpha> cond \<Rightarrow>('f,'\<alpha>) hrel_cp \<Right
 
 subsection{*GUARD*}
 
-abbreviation guard_c :: "'f \<Rightarrow> '\<alpha> cond \<Rightarrow> ('f,'\<alpha>) hrel_cp" (*Is this correct!*) 
-where "guard_c f b \<equiv>  (bif b then SKIP else (\<not>$abrupt\<acute> \<and> $fault\<acute> =\<^sub>u \<guillemotleft>Some f\<guillemotright> \<and> \<lceil>II\<rceil>\<^sub>C) eif)"
+abbreviation guard_c :: "'f \<Rightarrow> '\<alpha> cond \<Rightarrow> ('f,'\<alpha>) hrel_cp" 
+where "guard_c f b \<equiv>  
+      (bif b then SKIP else (\<not>$abrupt\<acute> \<and> \<not>$stuck\<acute> \<and> $fault\<acute> \<and> $fault_tr\<acute> =\<^sub>u \<guillemotleft>Some f\<guillemotright> \<and> \<lceil>II\<rceil>\<^sub>C) eif)"
 
 subsection{*assert and assume*}
 
