WP1-Programming-Languages-Semantics/WP11-C-semantics/src/IMP-Lenses/hoare/utp_hoare_total.thy
@@ -8,13 +8,15 @@ named_theorems hoare_total
 subsection {*Hoare triple definition*}
 
 definition hoare_rd :: "'\<alpha> cond \<Rightarrow> ('f,'\<alpha>) hrel_cp \<Rightarrow> '\<alpha> cond \<Rightarrow> bool" ("\<lbrace>_\<rbrace>_\<lbrace>_\<rbrace>\<^sub>D") where
-[upred_defs]:"\<lbrace>p\<rbrace>Q\<lbrace>r\<rbrace>\<^sub>D = ((\<lceil>p\<rceil>\<^sub>C\<^sub>< \<and> $ok \<and> \<not>$abrupt \<and> $fault =\<^sub>u \<guillemotleft>None\<guillemotright> \<Rightarrow> 
-                          \<lceil>r\<rceil>\<^sub>C\<^sub>> \<and> $ok\<acute> \<and> \<not>$abrupt\<acute> \<and> $fault\<acute> =\<^sub>u \<guillemotleft>None\<guillemotright>) \<sqsubseteq> Q)"
+[upred_defs]:"\<lbrace>p\<rbrace>Q\<lbrace>r\<rbrace>\<^sub>D = 
+  ((\<lceil>p\<rceil>\<^sub>C\<^sub>< \<and> $ok \<and> \<not>$abrupt \<and> \<not>$stuck \<and> \<not>$fault \<and> $fault_tr =\<^sub>u \<guillemotleft>None\<guillemotright> \<Rightarrow> 
+    \<lceil>r\<rceil>\<^sub>C\<^sub>> \<and> $ok\<acute> \<and> \<not>$abrupt\<acute> \<and> \<not>$stuck\<acute> \<and> \<not>$fault\<acute> \<and> $fault_tr\<acute> =\<^sub>u \<guillemotleft>None\<guillemotright>) \<sqsubseteq> Q)"
 
-lemma hoare_true [hoare_total]: 
-  assumes "ok\<sharp>\<sharp>C" "abrupt\<sharp>\<sharp>C" "fault\<sharp>\<sharp>C"
+lemma hoare_true_t [hoare_total]:
+  assumes "$ok \<sharp> C" "$abrupt \<sharp> C" "$stuck \<sharp> C" "$fault \<sharp> C" "$fault_tr \<sharp> C"
+          "$ok\<acute> \<sharp> C" "$abrupt\<acute> \<sharp> C" "$stuck\<acute> \<sharp> C" "$fault\<acute> \<sharp> C" "$fault_tr\<acute> \<sharp> C"
   shows "\<lbrace>p\<rbrace>C\<lbrace>true\<rbrace>\<^sub>D"
-  using assms oops
+ oops
 
 lemma hoare_false_t [hoare_total]: "\<lbrace>false\<rbrace>C\<lbrace>q\<rbrace>\<^sub>D"
   by rel_auto
@@ -60,14 +62,14 @@ subsection {*Hoare for Sequential Composition*}
 lemma seq_hoare_r_t [hoare_total]: 
   assumes"\<lbrace>p\<rbrace>C\<^sub>1\<lbrace>s\<rbrace>\<^sub>D" and "\<lbrace>s\<rbrace>C\<^sub>2\<lbrace>r\<rbrace>\<^sub>D" 
   shows"\<lbrace>p\<rbrace>C\<^sub>1 ;; C\<^sub>2\<lbrace>r\<rbrace>\<^sub>D"
-  by (insert assms) rel_blast
+  by (insert assms, rel_auto) metis+ 
 
 subsection {*Hoare for Conditional*}
 
 lemma cond_hoare_r_t [hoare_total]: 
   assumes "\<lbrace>b \<and> p\<rbrace>C\<^sub>1\<lbrace>q\<rbrace>\<^sub>D" and "\<lbrace>\<not>b \<and> p\<rbrace>C\<^sub>2\<lbrace>q\<rbrace>\<^sub>D" 
   shows "\<lbrace>p\<rbrace>C\<^sub>1 \<triangleleft> \<lceil>b\<rceil>\<^sub>C\<^sub>< \<triangleright> C\<^sub>2\<lbrace>q\<rbrace>\<^sub>D"
-  by (insert assms) rel_blast
+  by (insert assms, rel_auto) metis+ 
 
 subsection {*Hoare for assert*}
 
